secure_api/box/Box.PlainBox.fst
@@ -17,8 +17,7 @@ type bytes = seq UInt8.t
    The protected plaintext type of the pkae construction. It is associated with an id and bytes, that
    match the required format for encryption with the Salsa20 spec.
 *)
-noeq abstract type protected_pkae_plain =
-  | Prot_pkae_p: #i:id{AE_id? i} -> b:bytes{Seq.length b / Spec.Salsa20.blocklen < pow2 32} -> protected_pkae_plain
+abstract type protected_pkae_plain (i:id{AE_id? i}) = b:bytes{Seq.length b / Spec.Salsa20.blocklen < pow2 32}
 
 (**
    The unprotected plaintext type.
@@ -28,27 +27,26 @@ type pkae_plain = b:bytes{Seq.length b / Spec.Salsa20.blocklen < pow2 32}
 (**
    A helper function to get the index of the abstract, protected plaintext.
 *)
-val get_index: p:protected_pkae_plain -> Tot (i:id{i=p.i})
-let get_index p =
-  p.i
+val get_index: #i:id{AE_id? i} -> p:protected_pkae_plain i -> Tot (i:id)
+let get_index #i p =
+  i
 
 (**
    This function can bypass the abstraction protection of the protected plaintext type. However, this is only possible
    if pkae_ind_cpa is not idealized, or if the id associated with the plaintext is dishonest.
 *)
-val repr: p:protected_pkae_plain{not pkae_ind_cpa \/ (dishonest p.i) } -> Tot (b:pkae_plain{Seq.length b / Spec.Salsa20.blocklen < pow2 32})
-let repr p = p.b
+val repr: #i:id{AE_id? i} -> p:protected_pkae_plain i{not pkae_ind_cpa \/ dishonest i} -> Tot (b:pkae_plain{Seq.length b / Spec.Salsa20.blocklen < pow2 32})
+let repr #i p = p
 
 (**
    This function allows the creation of protected plaintexts. Protected plaintexts can only be created by the adversary if
    either pkae_int_ctxt is not idealized or of the id associated with the newly created plaintext is dishonest.
 *)
-val coerce: #i:id{AE_id? i} -> p:pkae_plain{not pkae_int_ctxt \/ (dishonest i)} -> Tot (prot:protected_pkae_plain{i=prot.i})
-let coerce #i p =
-  Prot_pkae_p #i p
+val coerce: #i:id{AE_id? i} -> p:pkae_plain{not pkae_int_ctxt \/ dishonest i} -> Tot (prot:protected_pkae_plain i)
+let coerce #i p = p
 
 (**
    A helper function to obtain the length of a protected plaintext.
 *)
-val length:  protected_pkae_plain -> Tot (n:nat{n / Spec.Salsa20.blocklen < pow2 32})
-let length p = Seq.length p.b
+val length: #i:id{AE_id? i} -> protected_pkae_plain i -> Tot (n:nat{n / Spec.Salsa20.blocklen < pow2 32})
+let length #i p = Seq.length p
